src/program_proof/tulip/invariance/prepare.v
@@ -1,0 +1,618 @@
+From Perennial.program_proof.tulip Require Import prelude.
+
+Lemma ext_by_cmtd_inv_prepare repl cmtd kmod ts :
+  kmod !! O = None ->
+  kmod !! ts = None ->
+  (length cmtd ≤ ts)%nat ->
+  ext_by_cmtd repl cmtd kmod O ->
+  ext_by_cmtd repl cmtd kmod ts.
+Proof.
+  intros Hz Hts Hlen Hdiff.
+  rewrite /ext_by_cmtd Hz in Hdiff.
+  destruct Hdiff as (rts & Hdiff & _).
+  rewrite /ext_by_cmtd Hts.
+  by eauto.
+Qed.
+
+Lemma prepared_impl_locked_inv_prepare stm ptsm ts pwrs :
+  stm !! O = None ->
+  dom pwrs ⊆ dom ptsm ->
+  set_Forall (λ k, ptsm !! k = Some O) (dom pwrs) ->
+  prepared_impl_locked stm ptsm ->
+  prepared_impl_locked (<[ts:=StPrepared pwrs]> stm) (acquire ts pwrs ptsm).
+Proof.
+  intros Hnz Hincl Hfree Hpil tsx pwrsx key Hpwrsx Hkey.
+  destruct (decide (tsx = ts)) as [-> | Hne]; last first.
+  { rewrite lookup_insert_ne in Hpwrsx; last done.
+    specialize (Hpil _ _ _ Hpwrsx Hkey).
+    destruct (pwrs !! key) as [v |] eqn:Hpwrs.
+    { exfalso.
+      assert (Htsxnz : tsx ≠ O).
+      { intros ->. by rewrite Hnz in Hpwrsx. }
+      apply elem_of_dom_2 in Hpwrs.
+      specialize (Hfree _ Hpwrs). simpl in Hfree.
+      rewrite Hfree in Hpil.
+      inv Hpil.
+    }
+    by rewrite acquire_unmodified.
+  }
+  rewrite lookup_insert in Hpwrsx.
+  inv Hpwrsx.
+  apply acquire_modified.
+  { by apply elem_of_dom. }
+  apply elem_of_dom.
+  set_solver.
+Qed.
+
+Lemma locked_impl_prepared_inv_prepare stm ptsm ts pwrs :
+  dom pwrs ⊆ dom ptsm ->
+  stm !! ts = None ->
+  locked_impl_prepared stm ptsm ->
+  locked_impl_prepared (<[ts:=StPrepared pwrs]> stm) (acquire ts pwrs ptsm).
+Proof.
+  intros Hincl Hnotin Hlip key tsx Htsx Hnz.
+  destruct (decide (tsx = ts)) as [-> | Hne]; last first.
+  { rewrite lookup_insert_ne; last done.
+    apply Hlip; last done.
+    destruct (pwrs !! key) as [v |] eqn:Hpwrs.
+    { exfalso.
+      rewrite acquire_modified in Htsx; [inv Htsx | done |].
+      apply elem_of_dom_2 in Hpwrs.
+      apply elem_of_dom.
+      set_solver.
+    }
+    by rewrite -Htsx acquire_unmodified.
+  }
+  exists pwrs.
+  rewrite lookup_insert.
+  split; first done.
+  (* Prove that before this transition no keys are locked by [ts]. *)
+  apply dec_stable.
+  intros Hkey.
+  apply not_elem_of_dom in Hkey.
+  rewrite acquire_unmodified in Htsx; last apply Hkey.
+  specialize (Hlip _ _ Htsx Hnz).
+  destruct Hlip as (pwrsx & Hpwrsx & _).
+  by rewrite Hpwrsx in Hnotin.
+Qed.
+
+Section inv.
+  Context `{!tulip_ghostG Σ}.
+
+  Lemma key_inv_not_committed γ p gid ts pm key kmodc tsprep :
+    gid = key_to_group key ->
+    pm !! ts = None ->
+    own_group_prepm γ gid pm -∗
+    txnsys_inv γ p -∗
+    key_inv_with_kmodc_no_tsprep γ key kmodc tsprep -∗
+    ⌜kmodc !! ts = None⌝.
+  Proof.
+    iIntros (Hgid Hnone) "Hpm Htxnsys Hkey".
+    do 2 iNamed "Htxnsys".
+    destruct (resm !! ts) as [res |] eqn:Hlookup.
+    { (* Case: Committed or aborted. *)
+      iDestruct (big_sepM_lookup with "Hvr") as "Hres"; first apply Hlookup.
+      destruct res.
+      { (* Case: Committed. *)
+        simpl.
+        destruct (wrs !! key) as [v |] eqn:Hkey.
+        { (* Case: [key] in the write set of [ts]; contradiction. *)
+          rewrite /all_prepared.
+          iDestruct "Hres" as "[_ Hpreps]".
+          iDestruct (big_sepS_elem_of _ _ gid with "Hpreps") as "Hprep".
+          { rewrite Hgid. by eapply elem_of_key_to_group_ptgroups, elem_of_dom_2. }
+          iDestruct (group_prep_lookup with "Hpm Hprep") as %Hprep.
+          congruence.
+        }
+        (* Case: [key] not in the write set of [ts]. *)
+        do 2 iNamed "Hkey".
+        iDestruct (cmtd_kmod_vslice_agree with "Hkmodcs Hkmodc") as %Hkmodc.
+        { apply Hall. }
+        iPureIntro.
+        subst kmodc.
+        by eapply vslice_resm_to_tmods_committed_absent.
+      }
+      { (* Case: Aborted. *)
+        do 2 iNamed "Hkey".
+        iDestruct (cmtd_kmod_vslice_agree with "Hkmodcs Hkmodc") as %Hkmodc.
+        { apply Hall. }
+        iPureIntro.
+        subst kmodc.
+        by eapply vslice_resm_to_tmods_aborted.
+      }
+    }
+    (* Case: Not committed or aborted. *)
+    do 2 iNamed "Hkey".
+    iDestruct (cmtd_kmod_vslice_agree with "Hkmodcs Hkmodc") as %Hkmodc.
+    { apply Hall. }
+    iPureIntro.
+    subst kmodc.
+    by eapply vslice_resm_to_tmods_not_terminated.
+  Qed.
+
+  Lemma keys_inv_not_committed γ p gid ts pm tspreps :
+    set_Forall (λ k, key_to_group k = gid) (dom tspreps) ->
+    pm !! ts = None ->
+    ([∗ map] key ↦ tsprep ∈ tspreps, key_inv_no_tsprep γ key tsprep) -∗
+    own_group_prepm γ gid pm -∗
+    txnsys_inv γ p -∗
+    ([∗ map] key ↦ tsprep ∈ tspreps, key_inv_xcmted_no_tsprep γ key tsprep ts) ∗
+    own_group_prepm γ gid pm ∗
+    txnsys_inv γ p.
+  Proof.
+    iIntros (Hgid Hnone) "Hkeys Hst Htxn".
+    iApply (big_sepM_impl_res with "Hkeys [Hst Htxn]").
+    { iFrame. } (* why can't $ do the work? *)
+    iIntros "!>" (k t Hkt) "Hkey [Hst Htxn]".
+    apply elem_of_dom_2 in Hkt.
+    specialize (Hgid _ Hkt). simpl in Hgid.
+    iDestruct (key_inv_no_tsprep_unseal_kmodc with "Hkey") as (kmodc) "Hkey".
+    iDestruct (key_inv_not_committed with "Hst Htxn Hkey") as %Hprep; first done.
+    { apply Hnone. }
+    iFrame "∗ %".
+  Qed.
+
+  Lemma key_inv_prepare {γ gid ts} pwrs k :
+    ts ≠ O ->
+    key_to_group k = gid ->
+    k ∈ dom pwrs ->
+    quorum_validated γ gid ts -∗
+    is_txn_pwrs γ gid ts pwrs -∗
+    key_inv_xcmted_no_tsprep γ k O ts -∗
+    ([∗ set] rid ∈ rids_all, replica_inv_xfinalized γ gid rid {[ts]}) -∗
+    key_inv_xcmted_no_tsprep γ k ts ts ∗
+    ([∗ set] rid ∈ rids_all, replica_inv_xfinalized γ gid rid {[ts]}).
+  Proof.
+    iIntros (Hnz Hgid Hk) "#Hqv #Hpwrs Hkey Hrps".
+    do 3 iNamed "Hkey".
+    destruct (decide (ts < pred (length cmtd))%nat) as [Hlt | Hge].
+    { (* From [Hqv] and [Hqpa] we obtain a replica that currently grants the
+         lock of [k] to [ts], but also has already validated or read [k] with a
+         larger timestamp. *)
+      iDestruct "Hqv" as (ridsq1) "[Hqv %Hq1]".
+      iDestruct "Hqvfb" as (ridsq2) "[Hqvfb %Hq2]".
+      pose proof (cquorums_overlapped _ _ _ Hq1 Hq2) as (rid & Hinq1 & Hinq2).
+      pose proof (cquorum_elem_of _ _ _ Hinq1 Hq1) as Hinall.
+      iDestruct (big_sepS_elem_of with "Hqv") as "Hrv"; first apply Hinq1.
+      iDestruct (big_sepS_elem_of with "Hqvfb") as "Hrvfb"; first apply Hinq2.
+      iDestruct (big_sepS_elem_of with "Hrps") as "Hrp"; first apply Hinall.
+      iNamed "Hrp".
+      iDestruct (replica_inv_xfinalized_validated_impl_prepared with "Hrv Hrp")
+        as (pwrs') "%Hpreped".
+      { apply Hxfinal. }
+      { set_solver. }
+      (* Prove [pwrs' = pwrs]. *)
+      iNamed "Hrp".
+      iDestruct (big_sepM_lookup with "Hsafep") as "Hpwrs'"; first apply Hpreped.
+      iDestruct (txn_pwrs_agree with "Hpwrs Hpwrs'") as %->.
+      (* Prove [k] is locked by [ts]. *)
+      specialize (Hpil _ _ _ Hpreped Hk).
+      (* Prove the validation list for [k] has extended beyond [length cmtd]. *)
+      iDestruct "Hrvfb" as (vdlb) "[Hvdlb %Hlen]".
+      assert (is_Some (kvdm !! k)) as [vd Hvd].
+      { pose proof (map_Forall2_dom_L _ _ _ Hlocked) as Hdom.
+        by rewrite -elem_of_dom Hdom elem_of_dom.
+      }
+      iDestruct (big_sepM_lookup with "Hkvdm") as "Hvd"; first apply Hvd.
+      rewrite Hgid.
+      iDestruct (replica_key_validation_prefix with "Hvdlb Hvd") as %Hprefix.
+      exfalso.
+      apply prefix_length in Hprefix.
+      pose proof (map_Forall2_lookup_Some _ _ _ _ _ _ Hvd Hpil Hlocked) as Hub.
+      specialize (Hub Hnz).
+      destruct Hub as [_ Hub].
+      clear -Hlt Hlen Hprefix Hub.
+      lia.
+    }
+    rewrite Nat.nlt_ge in Hge.
+    destruct (decide (ts = pred (length cmtd))) as [Heq | Hne].
+    { (* From [Hqv] and [Hcori] we obtain a replica that currently grants the
+         lock of [k] to [ts], but also has invalidated (through reading the key)
+         at [ts]. *)
+      rewrite /committed_or_quorum_invalidated -Heq Hnc.
+      iDestruct "Hqv" as (ridsq1) "[Hqv %Hq1]".
+      iDestruct "Hcori" as (ridsq2) "[Hcori %Hq2]".
+      pose proof (cquorums_overlapped _ _ _ Hq1 Hq2) as (rid & Hinq1 & Hinq2).
+      pose proof (cquorum_elem_of _ _ _ Hinq1 Hq1) as Hinall.
+      iDestruct (big_sepS_elem_of with "Hqv") as "Hrv"; first apply Hinq1.
+      iDestruct (big_sepS_elem_of with "Hcori") as "Hvdlb"; first apply Hinq2.
+      iDestruct (big_sepS_elem_of with "Hrps") as "Hrp"; first apply Hinall.
+      iNamed "Hrp".
+      iDestruct (replica_inv_xfinalized_validated_impl_prepared with "Hrv Hrp")
+        as (pwrs') "%Hpreped".
+      { apply Hxfinal. }
+      { set_solver. }
+      (* Prove [pwrs' = pwrs]. *)
+      iNamed "Hrp".
+      iDestruct (big_sepM_lookup with "Hsafep") as "Hpwrs'"; first apply Hpreped.
+      iDestruct (txn_pwrs_agree with "Hpwrs Hpwrs'") as %->.
+      (* Prove [k] is locked by [ts]. *)
+      specialize (Hpil _ _ _ Hpreped Hk).
+      assert (is_Some (kvdm !! k)) as [vd Hvd].
+      { pose proof (map_Forall2_dom_L _ _ _ Hlocked) as Hdom.
+        by rewrite -elem_of_dom Hdom elem_of_dom.
+      }
+      iDestruct (big_sepM_lookup with "Hkvdm") as "Hvd"; first apply Hvd.
+      rewrite Hgid.
+      pose proof (map_Forall2_lookup_Some _ _ _ _ _ _ Hvd Hpil Hlocked) as Hvts.
+      specialize (Hvts Hnz).
+      destruct Hvts as [Hvts _].
+      iDestruct (replica_key_validation_lookup with "Hvdlb Hvd") as %Hnvts.
+      by rewrite Hvts in Hnvts.
+    }
+    assert (Hle : (length cmtd ≤ ts)%nat) by lia.
+    iFrame "∗ # %".
+    iPureIntro.
+    by apply ext_by_cmtd_inv_prepare.
+  Qed.
+
+  Lemma keys_inv_prepare γ gid ts pwrs :
+    ts ≠ O ->
+    quorum_validated γ gid ts -∗
+    is_txn_pwrs γ gid ts pwrs -∗
+    ([∗ set] key ∈ dom pwrs, key_inv_xcmted_no_tsprep γ key O ts) -∗
+    ([∗ set] rid ∈ rids_all, replica_inv_xfinalized γ gid rid {[ts]}) -∗
+    ([∗ set] key ∈ dom pwrs, key_inv_xcmted_no_tsprep γ key ts ts) ∗
+    ([∗ set] rid ∈ rids_all, replica_inv_xfinalized γ gid rid {[ts]}).
+  Proof.
+    iIntros (Hnz) "#Hqv #Hpwrs Hkeys Hrps".
+    iAssert (⌜set_Forall (λ k, key_to_group k = gid) (dom pwrs)⌝)%I as %Hgroup.
+    { iDestruct "Hpwrs" as (wrs) "[Hwrs %Hpwrs]".
+      iPureIntro.
+      rewrite /wrs_group in Hpwrs.
+      intros k Hk.
+      apply elem_of_dom in Hk as [v Hv].
+      rewrite Hpwrs map_lookup_filter_Some in Hv.
+      by destruct Hv as [_ Hgid].
+    }
+    iApply (big_sepS_impl_res with "Hkeys Hrps").
+    iIntros (k Hk) "!> Hkey Hrps".
+    specialize (Hgroup _ Hk).
+    by iApply (key_inv_prepare with "Hqv Hpwrs Hkey Hrps").
+  Qed.
+
+  Lemma apply_cmds_cm_subseteq {log logp cm cmp histm histmp} :
+    prefix logp log ->
+    apply_cmds log = State cm histm ->
+    apply_cmds logp = State cmp histmp ->
+    cmp ⊆ cm.
+  Admitted.
+
+  Lemma replica_inv_not_finalized γ gid rid log cm hists tss ts :
+    cm !! ts = None ->
+    apply_cmds log = State cm hists ->
+    replica_inv_xfinalized γ gid rid tss -∗
+    own_txn_log_half γ gid log -∗
+    replica_inv_xfinalized γ gid rid ({[ts]} ∪ tss) ∗
+    own_txn_log_half γ gid log.
+  Proof.
+    iIntros (Hnone Happly) "Hrp Hlog".
+    iDestruct "Hrp" as (cmrp) "Hrp".
+    do 2 iNamed "Hrp".
+    iDestruct (txn_log_prefix with "Hlog Hclog") as %Hprefix.
+    pose proof (apply_cmds_cm_subseteq Hprefix Happly Hrsm) as Hincl.
+    iFrame "Hlog ∗ # %".
+    iPureIntro.
+    apply set_Forall_union; last apply Hxfinal.
+    rewrite set_Forall_singleton.
+    by eapply lookup_weaken_None.
+  Qed.
+
+  Lemma replicas_inv_not_finalized γ gid rids log cm hists ts :
+    cm !! ts = None ->
+    apply_cmds log = State cm hists ->
+    ([∗ set] rid ∈ rids, replica_inv γ gid rid) -∗
+    own_txn_log_half γ gid log -∗
+    ([∗ set] rid ∈ rids, replica_inv_xfinalized γ gid rid {[ts]}) ∗
+    own_txn_log_half γ gid log.
+  Proof.
+    iIntros (Hxfinal Happly) "Hrps Hlog".
+    iApply (big_sepS_impl_res with "Hrps Hlog").
+    iIntros (rid Hrid) "!> Hrp Hlog".
+    iDestruct (replica_inv_xfinalized_empty with "Hrp") as "Hrp".
+    iDestruct (replica_inv_not_finalized with "Hrp Hlog") as "[Hrp Hlog]".
+    { apply Hxfinal. }
+    { apply Happly. }
+    rewrite union_empty_r_L.
+    iFrame.
+  Qed.
+
+  Lemma replica_inv_exclude_concurrent_prepare γ gid rid tss ts1 ts2 pwrs1 pwrs2 :
+    ts1 ≠ ts2 ->
+    ts1 ∈ tss ->
+    ts2 ∈ tss ->
+    dom pwrs1 ∩ dom pwrs2 ≠ ∅ ->
+    is_replica_validated_ts γ gid rid ts1 -∗
+    is_replica_validated_ts γ gid rid ts2 -∗
+    is_txn_pwrs γ gid ts1 pwrs1 -∗
+    is_txn_pwrs γ gid ts2 pwrs2 -∗
+    replica_inv_xfinalized γ gid rid tss -∗
+    False.
+  Proof.
+    iIntros (Hne Hin1 Hin2 Hoverlap) "Hts1 Hts2 Hwrs1 Hwrs2 Hrp".
+    iNamed "Hrp".
+    iDestruct (replica_inv_xfinalized_validated_impl_prepared with "Hts1 Hrp")
+      as (pwrs1') "%Hpwrs1".
+    { apply Hxfinal. }
+    { apply Hin1. }
+    iDestruct (replica_inv_xfinalized_validated_impl_prepared with "Hts2 Hrp")
+      as (pwrs2') "%Hpwrs2".
+    { apply Hxfinal. }
+    { apply Hin2. }
+    iNamed "Hrp".
+    iAssert (⌜pwrs1' = pwrs1⌝)%I as %->.
+    { iDestruct (big_sepM_lookup with "Hsafep") as "Hsafe"; first apply Hpwrs1.
+      iApply (txn_pwrs_agree with "Hwrs1 Hsafe").
+    }
+    iAssert (⌜pwrs2' = pwrs2⌝)%I as %->.
+    { iDestruct (big_sepM_lookup with "Hsafep") as "Hsafe"; first apply Hpwrs2.
+      iApply (txn_pwrs_agree with "Hwrs2 Hsafe").
+    }
+    exfalso.
+    apply set_choose_L in Hoverlap as [k Hk].
+    apply elem_of_intersection in Hk as [Hinpwrs1 Hinpwrs2].
+    pose proof (Hpil _ _ _ Hpwrs1 Hinpwrs1) as Hts1.
+    pose proof (Hpil _ _ _ Hpwrs2 Hinpwrs2) as Hts2.
+    rewrite Hts1 in Hts2.
+    inv Hts2.
+  Qed.
+
+  Lemma repl_ts_acquire_disjoint {γ} ts wrs tss :
+    dom tss ## dom wrs ->
+    ([∗ map] k ↦ t ∈ tss, own_repl_ts_half γ k t) -∗
+    ([∗ map] k ↦ t ∈ acquire ts wrs tss, own_repl_ts_half γ k t).
+  Proof.
+    iIntros (Hdom) "Htpls".
+    iApply (big_sepM_impl_dom_eq with "Htpls"); first apply acquire_dom.
+    iIntros "!>" (k ts1 ts2 Hts1 Hts2) "Hts".
+    destruct (wrs !! k) as [v |] eqn:Hwrs.
+    { apply elem_of_dom_2 in Hts1. apply elem_of_dom_2 in Hwrs. set_solver. }
+    rewrite /acquire lookup_merge Hwrs Hts1 /= in Hts2.
+    by inv Hts2.
+  Qed.
+
+  Lemma group_inv_prepare γ p gid ts pwrs :
+    quorum_validated γ gid ts -∗
+    quorum_prepared γ gid ts -∗
+    safe_txn_pwrs γ gid ts pwrs -∗
+    txnsys_inv γ p -∗
+    ([∗ set] key ∈ keys_all, key_inv γ key) -∗
+    ([∗ set] rid ∈ rids_all, replica_inv γ gid rid) -∗
+    group_inv γ gid ==∗
+    txnsys_inv γ p ∗
+    ([∗ set] key ∈ keys_all, key_inv γ key) ∗
+    ([∗ set] rid ∈ rids_all, replica_inv γ gid rid) ∗
+    group_inv γ gid ∗
+    is_group_prepared γ gid ts.
+  Proof.
+    iIntros "#Hqv #Hqp #Hpwrs Htxnsys Hkeys Hrps Hgroup".
+    do 2 iNamed "Hgroup".
+    destruct (stm !! ts) as [st |] eqn:Hstm.
+    { (* Case: Txn [ts] has already prepared, aborted, or committed. *)
+      destruct st as [pwrs' | |].
+      { (* Case: Prepared. Simply take the [is_group_prepared] in [Hsafestm]. *)
+        iDestruct (big_sepM_lookup with "Hsafestm") as "#Hst"; first apply Hstm.
+        iDestruct "Hst" as "[Hpreped _]".
+        by iFrame "Htxnsys Hkeys Hrps ∗ # %".
+      }
+      { (* Case: Committed. Use stability to obtain [pm !! ts = true] and
+           extract a witness. Note that another way to prove this case is to
+           deduce preparedness from committedness. Having two ways to prove the
+           same thing might suggest something is redudant? *)
+        admit.
+      }
+      { (* Case: Aborted. Same as the committed case. Note that this case (i.e.,
+           not prepared but aborted) could indeed happen if another participant
+           group has aborted earlier. *)
+        admit.
+      }
+    }
+    (* Case: Txn [ts] has not prepared, aborted, or committed. *)
+    assert (Hnone : pm !! ts = None).
+    { apply not_elem_of_dom. apply not_elem_of_dom in Hstm. set_solver. }
+    (* Take the required keys invariants. *)
+    iDestruct "Hpwrs" as (wrs) "[Hwrs %Hpwrs]".
+    destruct Hpwrs as (Hvts & Hvwrs & Hnempty & Hpwrs).
+    iDestruct (big_sepS_subseteq_acc _ _ (dom pwrs) with "Hkeys") as "[Hkeys HkeysC]".
+    { (* Prove [dom pwrs ⊆ keys_all] *)
+      transitivity (dom wrs); last done.
+      rewrite Hpwrs.
+      apply dom_filter_subseteq.
+    }
+    (* Take the required prepare timestamps from the group invariant. *)
+    iDestruct (big_sepM_dom_subseteq_difference _ _ (dom pwrs) with "Hlocks")
+      as (tss [Hdom Hsubseteq]) "[Htss HlocksO]".
+    { (* Prove [dom pwrs ⊆ dom (filter_group gid tssg)]. *)
+      rewrite Hpwrs wrs_group_keys_group_dom filter_group_keys_group_dom Hdomptsm.
+      set_solver.
+    }
+    (* Expose the prepare timestamps from keys invariant. *)
+    iDestruct (keys_inv_extract_tsprep with "Hkeys") as (tssk) "(Hkeys & Htssk & %Hdom')".
+    (* Agree on the prepare timestamps from the group and keys invariants. *)
+    iDestruct (repl_ts_big_agree with "Htss Htssk") as %->; first by rewrite Hdom Hdom'.
+    clear Hdom'.
+    (* Update the prepare timestamps to [ts]. *)
+    set tss' := gset_to_gmap ts (dom tss).
+    iMod (repl_ts_big_update tss' with "Htss Htssk") as "[Htss Htssk]".
+    { by rewrite dom_gset_to_gmap. }
+    subst tss'.
+    (* Prove txn [ts] has not committed on [tpls]. *)
+    iDestruct (keys_inv_not_committed with "Hkeys Hpm Htxnsys") as "(Hkeys & Hpm & Htxn)".
+    { intros k Hk.
+      apply (key_to_group_filter_group _ _ tspreps).
+      apply subseteq_dom in Hsubseteq.
+      clear -Hsubseteq Hk. set_solver.
+    }
+    { apply Hnone. }
+    (* Prove that [ts] has not finalized on any replica. *)
+    assert (Hnotincm : cm !! ts = None).
+    { by rewrite Hcm lookup_omap Hstm. }
+    iDestruct (replicas_inv_not_finalized with "Hrps Hlog") as "[Hrps Hlog]".
+    { apply Hnotincm. }
+    { apply Hrsm. }
+    (* Prove that keys modified by [ts] are not prepared by another txn. *)
+    destruct (decide (map_Forall (λ _ t, t = O) tss)) as [Hallz | Hnz]; last first.
+    { (* Case: Some key [k] is locked. Derive contradiction. *)
+      apply map_not_Forall in Hnz as (k & pts & Hpts & Hnz); last apply _.
+      (* Prove [tspreps !! k = Some pts]. *)
+      unshelve epose proof (lookup_weaken _ tspreps _ _ Hpts _) as Hpts'.
+      { trans (filter_group gid tspreps); [apply Hsubseteq | apply map_filter_subseteq]. }
+      (* Obtain the write-set [pwrsx] of the conflicting txn [pts]. *)
+      specialize (Hlip _ _ Hpts' Hnz).
+      destruct Hlip as (pwrsx & Hpwrsx & Hinpwrsx).
+      (* Prove [ts ≠ pts]. *)
+      assert (Hne : ts ≠ pts).
+      { intros ->. by rewrite Hpwrsx in Hstm. }
+      (* From the fact that [pts] is prepared we obtain a quorum of nodes prepared for [pts]. *)
+      iDestruct (big_sepM_lookup with "Hsafestm") as "Hsafe"; first apply Hpwrsx.
+      iDestruct "Hsafe" as "[Hpreped Hsafe]".
+      iDestruct (group_prep_lookup with "Hpm Hpreped") as %Hpreped.
+      iDestruct (big_sepM_lookup with "Hsafepm") as "Hsafep"; first apply Hpreped.
+      iDestruct "Hsafep" as "[_ Hqv']".
+      (* Obtain two quorums from [Hqv] and [Hqv']. *)
+      iDestruct "Hqv" as (ridsq1) "[Hvd1 %Hridsq1]".
+      iDestruct "Hqv'" as (ridsq2) "[Hvd2 %Hridsq2]".
+      (* Exhibit the replica that has prepared for both [ts] and [pts]. *)
+      unshelve epose proof (quorums_overlapped rids_all ridsq1 ridsq2 _ _)
+        as (rid & Hin1 & Hin2); [by left | by left |].
+      iDestruct (big_sepS_elem_of with "Hvd1") as "Hvts"; first apply Hin1.
+      iDestruct (big_sepS_elem_of with "Hvd2") as "Hvpts"; first apply Hin2.
+      (* Obtain the replica invariant for [rid]. *)
+      pose proof (cquorum_elem_of _ _ _ Hin1 Hridsq1) as Hin.
+      iDestruct (big_sepS_elem_of with "Hrps") as "Hrp"; first apply Hin.
+      (* Prove that [pts] also has not finalized on [rid]. *)
+      assert (Hnotincmx : cm !! pts = None).
+      { by rewrite Hcm lookup_omap Hpwrsx. }
+      iDestruct (replica_inv_not_finalized with "Hrp Hlog") as "[Hrp Hlog]".
+      { apply Hnotincmx. }
+      { apply Hrsm. }
+      iAssert (is_txn_pwrs γ gid ts pwrs)%I as "Hpwrs".
+      { iFrame "Hwrs %". }
+      iDestruct (safe_txn_pwrs_impl_is_txn_pwrs with "Hsafe") as "Hpwrsx".
+      iDestruct (replica_inv_exclude_concurrent_prepare with "Hvts Hvpts Hpwrs Hpwrsx Hrp") as %[].
+      { apply Hne. }
+      { set_solver. }
+      { set_solver. }
+      { apply elem_of_dom_2 in Hpts.
+        rewrite Hdom in Hpts.
+        clear -Hpts Hinpwrsx. set_solver.
+      }
+    }
+    (* Case: All keys are free. Encode this fact into the key invariants. *)
+    iAssert ([∗ set] key ∈ dom tss, key_inv_xcmted_no_tsprep γ key O ts)%I
+      with "[Hkeys]" as "Hkeys".
+    { iApply (big_sepM_sepS_impl with "Hkeys"); first done.
+      iIntros (k pts Hpts) "!> Hkey".
+      specialize (Hallz _ _ Hpts). simpl in Hallz.
+      by subst pts.
+    }
+    (* Re-establish keys invariant w.r.t. updated tuples. *)
+    rewrite Hdom.
+    iDestruct (keys_inv_prepare with "Hqv [] Hkeys Hrps") as "[Hkeys Hrps]".
+    { rewrite /valid_ts in Hvts. lia. }
+    { iFrame "Hwrs %". }
+    (* Put ownership of prepare timestamp back to keys invariant. *)
+    iDestruct (keys_inv_merge_tsprep (dom pwrs) with "[Hkeys] Htssk") as "Hkeys".
+    { by rewrite dom_gset_to_gmap. }
+    { iApply (big_sepS_sepM_impl with "Hkeys"); first by rewrite dom_gset_to_gmap.
+      iIntros (k t Hkt) "!> Hkey".
+      apply lookup_gset_to_gmap_Some in Hkt as [_ ->].
+      do 2 iNamed "Hkey".
+      iFrame.
+    }
+    (* Merge the updated keys invariant back. *)
+    iDestruct ("HkeysC" with "Hkeys") as "Hkeys".
+    (* Merge ownership of tuples back to group invariants. *)
+    iAssert ([∗ map] k ↦ x ∈ filter_group gid (acquire ts pwrs tspreps), own_repl_ts_half γ k x)%I
+      with "[HlocksO Htss]" as "Hlocks".
+    { iDestruct (repl_ts_acquire_disjoint ts pwrs with "HlocksO") as "HlocksO".
+      { clear -Hdom. set_solver. }
+      rewrite acquire_difference_distr.
+      replace (gset_to_gmap _ _) with (acquire ts pwrs tss); last first.
+      { apply map_eq.
+        intros k.
+        destruct (pwrs !! k) as [v |] eqn:Hk.
+        { rewrite acquire_modified; last first.
+          { apply elem_of_dom_2 in Hk.
+            by rewrite -elem_of_dom Hdom.
+          }
+          { done. }
+          symmetry.
+          rewrite lookup_gset_to_gmap_Some.
+          by apply elem_of_dom_2 in Hk.
+        }
+        rewrite acquire_unmodified; last apply Hk.
+        replace (tss !! k) with (None : option nat); last first.
+        { symmetry. by rewrite -not_elem_of_dom Hdom not_elem_of_dom. }
+        symmetry.
+        rewrite lookup_gset_to_gmap_None.
+        by apply not_elem_of_dom.
+      }
+      iDestruct (big_sepM_subseteq_difference_2 with "Htss HlocksO") as "Hlocks".
+      { by apply acquire_mono. }
+      by rewrite acquire_filter_group_commute.
+    }
+    (* Insert [(ts, true)] into the prepare map and extract a witness. *)
+    iMod (group_prep_insert ts true with "Hpm") as "[Hpm #Hpreped]"; first apply Hnone.
+    (* Re-establish [safe_txnst] w.r.t. new status map. *)
+    iAssert ([∗ map] ts ↦ st ∈ <[ts := StPrepared pwrs]> stm, safe_txnst γ gid ts st)%I
+      as "Hsafestm'".
+    { iApply big_sepM_insert_2; last done.
+      by iFrame "Hwrs Hpreped".
+    }
+    iClear "Hsafestm".
+    (* Re-establish [safe_prep] w.r.t. new prepare map. *)
+    iAssert ([∗ map] ts ↦ p ∈ <[ts := true]> pm, safe_prep γ gid ts p)%I as "Hsafepm'".
+    { iApply big_sepM_insert_2; last done.
+      iFrame "Hqv Hqp".
+    }
+    iClear "Hsafepm".
+    iFrame "∗ # %".
+    iModIntro.
+    iSplit.
+    { iApply (big_sepS_mono with "Hrps").
+      iIntros (rid Hrid) "Hrp".
+      iNamed "Hrp".
+      iFrame.
+    }
+    iPureIntro.
+    assert (Hincl : dom pwrs ⊆ dom tspreps).
+    { rewrite Hdomptsm.
+      trans (dom wrs); last apply Hvwrs.
+      rewrite Hpwrs. apply dom_filter_subseteq.
+    }
+    split.
+    { rewrite 2!dom_insert_L. clear -Hdompm. set_solver. }
+    split.
+    { by rewrite acquire_dom. }
+    split.
+    { rewrite omap_insert_None; last done.
+      by rewrite -Hcm delete_notin.
+    }
+    split.
+    { apply prepared_impl_locked_inv_prepare.
+      { apply Htsnz. }
+      { apply Hincl. }
+      { intros k Hk.
+        rewrite -Hdom elem_of_dom in Hk.
+        destruct Hk as [t Ht].
+        specialize (Hallz _ _ Ht). simpl in Hallz. subst t.
+        eapply lookup_weaken; first apply Ht.
+        trans (filter_group gid tspreps); first apply Hsubseteq.
+        apply map_filter_subseteq.
+      }
+      { apply Hpil. }
+    }
+    split.
+    { apply locked_impl_prepared_inv_prepare.
+      { apply Hincl. }
+      { apply Hstm. }
+      { apply Hlip. }
+    }
+    { rewrite lookup_insert_ne; first apply Htsnz.
+      rewrite /valid_ts in Hvts.
+      lia.
+    }
+  Admitted.
+
+End inv.
