src/program_proof/tulip/res_replica.v
@@ -1,0 +1,129 @@
+(** Global resources. *)
+From Perennial.program_proof Require Import grove_prelude.
+From Perennial.program_proof.tulip Require Import base stability.
+
+Section res.
+  Context `{!tulip_ghostG Σ}.
+  (* TODO: remove this once we have real defintions for resources. *)
+  Implicit Type (γ : tulip_names).
+
+  Section replica_validated_ts.
+
+    (** Set of transaction IDs that are validated on a replica in a group. *)
+
+    Definition own_replica_validated_tss γ (gid rid : u64) (vtss : gset nat) : iProp Σ.
+    Admitted.
+
+    Definition is_replica_validated_ts γ (gid rid : u64) (vts : nat) : iProp Σ.
+    Admitted.
+
+    #[global]
+    Instance is_replica_validated_persistent γ gid rid ts :
+      Persistent (is_replica_validated_ts γ gid rid ts).
+    Admitted.
+
+    Lemma replica_validated_ts_insert γ gid rid vtss vts :
+      own_replica_validated_tss γ gid rid vtss ==∗
+      own_replica_validated_tss γ gid rid ({[vts]} ∪ vtss).
+    Admitted.
+
+    Lemma replica_validated_ts_witness γ gid rid vtss vts :
+      vts ∈ vtss ->
+      own_replica_validated_tss γ gid rid vtss -∗
+      is_replica_validated_ts γ gid rid vts.
+    Admitted.
+
+    Lemma replica_validated_ts_elem_of γ gid rid vtss vts :
+      is_replica_validated_ts γ gid rid vts -∗
+      own_replica_validated_tss γ gid rid vtss -∗
+      ⌜vts ∈ vtss⌝.
+    Admitted.
+
+  End replica_validated_ts.
+
+  Section replica_key_validation.
+
+    (** Mapping from keys to boolean lists encoding whether each key is
+    validated at a particular timestamp. *)
+
+    Definition own_replica_key_validation
+      γ (gid rid : u64) (key : dbkey) (l : list bool) : iProp Σ.
+    Admitted.
+
+    Definition is_replica_key_validation_lb
+      γ (gid rid : u64) (key : dbkey) (l : list bool) : iProp Σ.
+    Admitted.
+
+    Definition is_replica_key_validation_length_lb
+      γ (gid rid : u64) (key : dbkey) (n : nat) : iProp Σ :=
+      ∃ l, is_replica_key_validation_lb γ gid rid key l ∧ ⌜n ≤ length l⌝.
+
+    Definition is_replica_key_validation_at
+      γ (gid rid : u64) (key : dbkey) (ts : nat) (b : bool) : iProp Σ :=
+      ∃ l, is_replica_key_validation_lb γ gid rid key l ∧ ⌜l !! ts = Some b⌝.
+
+    Definition is_replica_key_validated_at
+      γ (gid rid : u64) (key : dbkey) (ts : nat) : iProp Σ :=
+      is_replica_key_validation_at γ gid rid key ts true.
+
+    Definition is_replica_key_invalidated_at
+      γ (gid rid : u64) (key : dbkey) (ts : nat) : iProp Σ :=
+      is_replica_key_validation_at γ gid rid key ts false.
+
+    #[global]
+    Instance is_replica_key_validation_lb_persistent γ gid rid key l :
+      Persistent (is_replica_key_validation_lb γ gid rid key l).
+    Admitted.
+
+    Lemma replica_key_validation_update {γ gid rid key l} l' :
+      prefix l l' ->
+      own_replica_key_validation γ gid rid key l ==∗
+      own_replica_key_validation γ gid rid key l'.
+    Admitted.
+
+    Lemma replica_key_validation_witness γ gid rid key l :
+      own_replica_key_validation γ gid rid key l -∗
+      is_replica_key_validation_lb γ gid rid key l.
+    Admitted.
+
+    Lemma replica_key_validation_prefix γ gid rid key l lb :
+      is_replica_key_validation_lb γ gid rid key lb -∗
+      own_replica_key_validation γ gid rid key l -∗
+      ⌜prefix lb l⌝.
+    Admitted.
+
+    Lemma replica_key_validation_lookup γ gid rid key l ts b :
+      is_replica_key_validation_at γ gid rid key ts b -∗
+      own_replica_key_validation γ gid rid key l -∗
+      ⌜l !! ts = Some b⌝.
+    Proof.
+      iIntros "(%lb & Hlb & %Hb) Hl".
+      iDestruct (replica_key_validation_prefix with "Hlb Hl") as %Hprefix.
+      iPureIntro.
+      by eapply prefix_lookup_Some.
+    Qed.
+
+  End replica_key_validation.
+
+  Section replica_ballot.
+
+    (** Mapping from transaction IDs to whether they are prepared on a replica
+    in a group at a certain rank. *)
+
+    Definition own_replica_ballots γ (gid rid : u64) (bs : gmap nat ballot) : iProp Σ.
+    Admitted.
+
+    Definition is_replica_ballot_lb γ (gid rid : u64) (ts : nat) (blt : ballot) : iProp Σ.
+    Admitted.
+
+    #[global]
+    Instance is_replica_ballot_lb_persistent γ gid rid ts blt :
+      Persistent (is_replica_ballot_lb γ gid rid ts blt).
+    Admitted.
+
+    Definition is_replica_pdec_at_rank γ (gid rid : u64) (ts rank : nat) (p : bool) : iProp Σ :=
+      ∃ blt, is_replica_ballot_lb γ gid rid ts blt ∧ ⌜blt !! rank = Some (Accept p)⌝.
+
+  End replica_ballot.
+
+End res.
