src/program_proof/tulip/stability.v
@@ -1,0 +1,9 @@
+From Perennial.program_proof Require Import grove_prelude.
+From Perennial.program_proof.rsm.pure Require Import quorum list.
+From Perennial.program_proof.tulip Require Import base.
+
+Inductive vote :=
+| Accept (p : bool)
+| Reject.
+
+Definition ballot := list vote.
